# Problem set 4


## The Kernel Perceptron Algorithm



### How the Kernel Perceptron Algorithm Works: Initalization

Recall that the original Perceptron Algorithm is given as the following:


Perceptron ({(ğ‘¥(ğ‘–),ğ‘¦(ğ‘–)),ğ‘–=1,...,ğ‘›},ğ‘‡): 
â€ƒâ€ƒinitialize  ğœƒ=0  (vector);
â€ƒâ€ƒâ€ƒâ€ƒfor  ğ‘¡=1,...,ğ‘‡ ,
â€ƒâ€ƒâ€ƒâ€ƒâ€ƒâ€ƒfor  ğ‘–=1,...,ğ‘› ,
â€ƒâ€ƒâ€ƒâ€ƒâ€ƒâ€ƒâ€ƒâ€ƒif  ğ‘¦(ğ‘–)(ğœƒâ‹…ğ‘¥(ğ‘–))â‰¤0 ,
â€ƒâ€ƒâ€ƒâ€ƒâ€ƒâ€ƒâ€ƒâ€ƒthen update  ğœƒ=ğœƒ+ğ‘¦(ğ‘–)ğ‘¥(ğ‘–). 

In the lecture, it was introduced that we can always express  ğœƒ  as

 	 ğœƒ=âˆ‘ğ‘—=1ğ‘›ğ›¼ğ‘—ğ‘¦(ğ‘—)ğœ™(ğ‘¥(ğ‘—)) 	 	 
where values of  ğ›¼1,â€¦,ğ›¼ğ‘›  may vary at each step of the algorithm. In other words, we can reformulate the algorithm so that we somehow initialize and update  ğ›¼ğ‘— 's, instead of  ğœƒ .

The reformulated algorithm, or kernel perceptron , can be given in the following form:


Kernel Perceptron ({(ğ‘¥(ğ‘–),ğ‘¦(ğ‘–)),ğ‘–=1,...,ğ‘›,ğ‘‡}) 
â€ƒâ€ƒInitialize  ğ›¼1,ğ›¼2,...,ğ›¼ğ‘›  to some values;
â€ƒâ€ƒfor  ğ‘¡=1,...,ğ‘‡ 
â€ƒâ€ƒâ€ƒâ€ƒfor  ğ‘–=1,...,ğ‘› 
â€ƒâ€ƒâ€ƒâ€ƒâ€ƒâ€ƒif  (Mistake Condition Expressed in ğ›¼ğ‘—) 
â€ƒâ€ƒâ€ƒâ€ƒâ€ƒâ€ƒâ€ƒâ€ƒUpdate  ğ›¼ğ‘—  appropriately

Look at the initialization statement of the algorithm. Which of the following is an equivalent way to initialize  ğ›¼1,ğ›¼2,...,ğ›¼ğ‘› , if we want the same result as initializing  ğœƒ=0 ?

Answer =  ğ›¼1=...=ğ›¼ğ‘›=0


### How the Kernel Perceptron Algorithm Works: The Update

As in the previous problem, our goal is to correctly reformulate the original perceptron algorithm. In other words, we want the algorithm to be about updating  ğ›¼ğ‘— 's instead of  ğœƒ .


Kernel Perceptron ({(ğ‘¥(ğ‘–),ğ‘¦(ğ‘–)),ğ‘–=1,...,ğ‘›,ğ‘‡}) 
â€ƒâ€ƒinitialize  ğ›¼1,ğ›¼2,...,ğ›¼ğ‘›  to some values;
â€ƒâ€ƒfor  ğ‘¡=1,...,ğ‘‡ 
â€ƒâ€ƒâ€ƒâ€ƒfor  ğ‘–=1,...,ğ‘› 
â€ƒâ€ƒâ€ƒâ€ƒâ€ƒâ€ƒif  (Mistake Condition Expressed in ğ›¼ğ‘—) 
â€ƒâ€ƒâ€ƒâ€ƒâ€ƒâ€ƒâ€ƒâ€ƒUpdate  ğ›¼ğ‘—  appropriately

Now look at the line "Update  ğ›¼ğ‘—  appropriately" in the above algorithm. Remember that we express  ğœƒ  as

ğœƒ=âˆ‘ğ‘—=1ğ‘›ğ›¼ğ‘—ğ‘¦(ğ‘—)ğœ™(ğ‘¥(ğ‘—)) 
 
Assuming that there was a mistake in classifying the  ğ‘– th data point i.e.

ğ‘¦(ğ‘–)(ğœƒâ‹…ğ‘¥(ğ‘–))â‰¤0 
 
which of the following conditions about  ğ›¼1,...,ğ›¼ğ‘›  is equivalent to

ğœƒ=ğœƒ+ğ‘¦(ğ‘–)ğœ™(ğ‘¥(ğ‘–)), 
 
the update condition of the original algorithm?


Answer = ğ›¼ğ‘–=ğ›¼ğ‘–+1

### How the Kernel Perceptron Algorithm Works: The Mistake Condition


Kernel Perceptron({(ğ‘¥(ğ‘–),ğ‘¦(ğ‘–)),ğ‘–=1,...,ğ‘›,ğ‘‡})
â€ƒâ€ƒinitialize ğ›¼1,ğ›¼2,...,ğ›¼ğ‘› to some values;
â€ƒâ€ƒfor ğ‘¡=1,...,ğ‘‡
â€ƒâ€ƒâ€ƒâ€ƒfor ğ‘–=1,...,ğ‘›
â€ƒâ€ƒâ€ƒâ€ƒâ€ƒâ€ƒif (Mistake Condition Expressed in ğ›¼ğ‘—)
â€ƒâ€ƒâ€ƒâ€ƒâ€ƒâ€ƒâ€ƒâ€ƒUpdate ğ›¼ğ‘— appropriately

Now look at the line "Mistake Condition Expressed in ğ›¼ğ‘—" in the above algorithm. Remember that we express ğœƒ as

ğœƒ=âˆ‘ğ‘—=1ğ‘›ğ›¼ğ‘—ğ‘¦(ğ‘—)ğœ™(ğ‘¥(ğ‘—))
 
Which of the following conditions is equivalent to ğ‘¦(ğ‘–)(ğœƒâ‹…ğœ™(ğ‘¥(ğ‘–)))â‰¤0? Remember from the video lecture above that given feature vectors ğœ™(ğ‘¥) and ğœ™(ğ‘¥â€²), we define the Kernel function ğ¾ as

ğ¾(ğ‘¥,ğ‘¥â€²)=ğœ™(ğ‘¥)ğœ™(ğ‘¥â€²).

Answer = ğ‘¦(ğ‘–)âˆ‘ğ‘›ğ‘—=1ğ›¼ğ‘—ğ‘¦(ğ‘—)ğ¾(ğ‘¥ğ‘—,ğ‘¥ğ‘–)â‰¤0


